compiler/src/DivisibleBy4.v
@@ -24,7 +24,11 @@ Ltac divisibleBy4_pre :=
   repeat match goal with
          | |- _ mod 4 = 0 -> _ => intro
          end;
-  repeat (rewrite ?word.unsigned_add, ?word.unsigned_mul, ?word.unsigned_of_Z || unfold word.wrap).
+  repeat (rewrite ?word.unsigned_add,
+                  ?word.unsigned_sub,
+                  ?word.unsigned_mul,
+                  ?word.unsigned_of_Z
+          || unfold word.wrap).
 
 Ltac solve_divisibleBy4 := divisibleBy4_pre; solve_mod4_0.
 
